src/core/DY.Core.Trace.Invariant.fst
@@ -87,8 +87,8 @@ let trace_event_invariant #invs tr event =
   | MsgSent msg ->
     // Messages sent on the network are publishable
     is_publishable tr msg
-  | SetState prin sess_id content -> (
-    // Stored states satisfy the custom state predicate
+  | SetVersion prin sess_id content -> (
+    // Stored versions satisfy the custom state predicate
     invs.trace_invs.state_pred.pred tr prin sess_id content
   )
   | Event prin tag content -> (
@@ -155,41 +155,41 @@ let msg_sent_on_network_are_publishable #invs tr msg =
     event_at_implies_trace_event_invariant tr i (MsgSent msg)
   )
 
-/// States stored satisfy the custom state predicate.
+/// Versions stored satisfy the custom state predicate.
 
-val state_was_set_implies_pred:
+val version_was_set_implies_pred:
   {|protocol_invariants|} -> tr:trace ->
   prin:principal -> sess_id:nat -> content:bytes ->
   Lemma
   (requires
     trace_invariant tr /\
-    state_was_set tr prin sess_id content
+    version_was_set tr prin sess_id content
   )
   (ensures state_pred tr prin sess_id content)
-  [SMTPat (state_was_set tr prin sess_id content);
+  [SMTPat (version_was_set tr prin sess_id content);
    SMTPat (trace_invariant tr);
   ]
-let state_was_set_implies_pred #invs tr prin sess_id content =
-  eliminate exists i. event_at tr i (SetState prin sess_id content)
+let version_was_set_implies_pred #invs tr prin sess_id content =
+  eliminate exists i. event_at tr i (SetVersion prin sess_id content)
   returns invs.trace_invs.state_pred.pred tr prin sess_id content
   with _. (
-    event_at_implies_trace_event_invariant tr i (SetState prin sess_id content);
+    event_at_implies_trace_event_invariant tr i (SetVersion prin sess_id content);
     invs.trace_invs.state_pred.pred_later (prefix tr i) tr prin sess_id content
   )
 
-/// States stored are knowable by the corresponding principal and state identifier.
+/// Versions stored are knowable by the corresponding principal and session identifier.
 // (This is a key lemma for attacker theorem.)
 
-val state_is_knowable_by:
+val version_is_knowable_by:
   {|protocol_invariants|} -> tr:trace ->
   prin:principal -> sess_id:nat -> content:bytes ->
   Lemma
   (requires
     trace_invariant tr /\
-    state_was_set tr prin sess_id content
+    version_was_set tr prin sess_id content
   )
   (ensures is_knowable_by (principal_state_label prin sess_id) tr content)
-let state_is_knowable_by #invs tr prin sess_id content =
+let version_is_knowable_by #invs tr prin sess_id content =
   state_pred_knowable tr prin sess_id content
 
 /// Triggered protocol events satisfy the event predicate.
