src/lib/state/DY.Lib.State.Typed.fst
@@ -5,16 +5,16 @@ open DY.Core
 open DY.Lib.Comparse.Glue
 open DY.Lib.State.Tagged
 
-class local_state (a:Type0) = {
+class local_version (a:Type0) = {
   tag: string;
   [@@@FStar.Tactics.Typeclasses.tcinstance]
   format: parseable_serializeable bytes a;
 }
 
-val mk_local_state_instance:
+val mk_local_version_instance:
   #a:Type0 -> {|parseable_serializeable bytes a|} -> string ->
-  local_state a
-let mk_local_state_instance #a #format tag = {
+  local_version a
+let mk_local_version_instance #a #format tag = {
   tag;
   format;
 }
@@ -61,39 +61,39 @@ let local_state_predicate_to_local_bytes_state_predicate #cinvs #a #ps_a tspred 
   }
 
 val has_local_state_predicate:
-  #a:Type -> {|local_state a|} ->
+  #a:Type -> {|local_version a|} ->
   invs:protocol_invariants -> local_state_predicate a ->
   prop
 let has_local_state_predicate #a #ls invs spred =
   has_local_bytes_state_predicate invs (ls.tag, (local_state_predicate_to_local_bytes_state_predicate spred))
 
 [@@ "opaque_to_smt"]
-val state_was_set:
-  #a:Type -> {|local_state a|} ->
+val version_was_set:
+  #a:Type -> {|local_version a|} ->
   trace -> principal -> nat -> a ->
   prop
-let state_was_set #a #ls tr prin sess_id content =
-  tagged_state_was_set tr ls.tag prin sess_id (serialize _ content)
+let version_was_set #a #ls tr prin sess_id content =
+  tagged_version_was_set tr ls.tag prin sess_id (serialize _ content)
 
 [@@ "opaque_to_smt"]
-val set_state:
-  #a:Type -> {|local_state a|} ->
+val set_version:
+  #a:Type -> {|local_version a|} ->
   principal -> nat -> a -> traceful unit
-let set_state #a #ls prin sess_id content =
-  set_tagged_state ls.tag prin sess_id (serialize _ content)
+let set_version #a #ls prin sess_id content =
+  set_tagged_version ls.tag prin sess_id (serialize _ content)
 
 [@@ "opaque_to_smt"]
-val get_state:
-  #a:Type -> {|local_state a|} ->
+val get_latest_version:
+  #a:Type -> {|local_version a|} ->
   principal -> nat -> traceful (option a)
-let get_state #a #ls prin sess_id =
-  let*? content_bytes = get_tagged_state ls.tag prin sess_id in
+let get_latest_version #a #ls prin sess_id =
+  let*? content_bytes = get_latest_tagged_version ls.tag prin sess_id in
   match parse a content_bytes with
   | None -> return None
   | Some content -> return (Some content)
 
-val set_state_invariant:
-  #a:Type -> {|local_state a|} ->
+val set_version_invariant:
+  #a:Type -> {|local_version a|} ->
   {|invs:protocol_invariants|} ->
   spred:local_state_predicate a ->
   prin:principal -> sess_id:nat -> content:a -> tr:trace ->
@@ -104,20 +104,20 @@ val set_state_invariant:
     has_local_state_predicate invs spred
   )
   (ensures (
-    let ((), tr_out) = set_state prin sess_id content tr in
+    let ((), tr_out) = set_version prin sess_id content tr in
     trace_invariant tr_out /\
-    state_was_set tr_out prin sess_id content
+    version_was_set tr_out prin sess_id content
   ))
-  [SMTPat (set_state prin sess_id content tr);
+  [SMTPat (set_version prin sess_id content tr);
    SMTPat (trace_invariant tr);
    SMTPat (has_local_state_predicate invs spred)]
-let set_state_invariant #a #ls #invs spred prin sess_id content tr =
-  reveal_opaque (`%set_state) (set_state #a);
-  reveal_opaque (`%state_was_set) (state_was_set #a);
+let set_version_invariant #a #ls #invs spred prin sess_id content tr =
+  reveal_opaque (`%set_version) (set_version #a);
+  reveal_opaque (`%version_was_set) (version_was_set #a);
   parse_serialize_inv_lemma #bytes a content
 
-val get_state_invariant:
-  #a:Type -> {|local_state a|} ->
+val get_latest_version_invariant:
+  #a:Type -> {|local_version a|} ->
   {|invs:protocol_invariants|} ->
   spred:local_state_predicate a ->
   prin:principal -> sess_id:nat -> tr:trace ->
@@ -127,7 +127,7 @@ val get_state_invariant:
     has_local_state_predicate invs spred
   )
   (ensures (
-    let (opt_content, tr_out) = get_state prin sess_id tr in
+    let (opt_content, tr_out) = get_latest_version prin sess_id tr in
     tr == tr_out /\ (
       match opt_content with
       | None -> True
@@ -136,28 +136,28 @@ val get_state_invariant:
       )
     )
   ))
-  [SMTPat (get_state #a prin sess_id tr);
+  [SMTPat (get_latest_version #a prin sess_id tr);
    SMTPat (trace_invariant tr);
    SMTPat (has_local_state_predicate invs spred)]
-let get_state_invariant #a #ls #invs spred prin sess_id tr =
-  reveal_opaque (`%get_state) (get_state #a)
+let get_latest_version_invariant #a #ls #invs spred prin sess_id tr =
+  reveal_opaque (`%get_latest_version) (get_latest_version #a)
 
-val state_was_set_implies_pred:
-  #a:Type -> {|local_state a|} ->
+val version_was_set_implies_pred:
+  #a:Type -> {|local_version a|} ->
   invs:protocol_invariants -> tr:trace ->
   spred:local_state_predicate a ->
   prin:principal -> sess_id:nat -> content:a ->
   Lemma
   (requires
-    state_was_set tr prin sess_id content /\
+    version_was_set tr prin sess_id content /\
     trace_invariant tr /\
     has_local_state_predicate invs spred
   )
   (ensures spred.pred tr prin sess_id content)
-  [SMTPat (state_was_set tr prin sess_id content);
+  [SMTPat (version_was_set tr prin sess_id content);
    SMTPat (trace_invariant tr);
    SMTPat (has_local_state_predicate invs spred);
   ]
-let state_was_set_implies_pred #a #ls invs tr spred prin sess_id content =
+let version_was_set_implies_pred #a #ls invs tr spred prin sess_id content =
   parse_serialize_inv_lemma #bytes a content;
-  reveal_opaque (`%state_was_set) (state_was_set #a)
+  reveal_opaque (`%version_was_set) (version_was_set #a)
